formal/Formal/Invariants.lean
@@ -5,6 +5,11 @@ namespace Silkworm
 
 theorem handle_no_callback_output_noop (st : EngineState) :
     handleCallbackOutput CallbackOutput.none st = st := by
-  simp [handleCallbackOutput, normalizeCallbackOutput, handleEvents, handleEventsWith]
+  simp [
+    handleCallbackOutput,
+    handleCallbackOutputWith,
+    normalizeCallbackOutput,
+    handleEventsWith,
+  ]
 
 end Silkworm
